Little tweak to prop_right_solve;  better handling of extern initialized arrays

floyd/globals_lemmas.v
@@ -3,6 +3,7 @@ Require Import floyd.client_lemmas.
 Require Import floyd.field_mapsto.
 Require Import floyd.assert_lemmas.
 Require Import floyd.malloc_lemmas.
+Require Import floyd.array_lemmas.
 Local Open Scope logic.
 
 Fixpoint fold_right_sepcon' (l: list(environ->mpred)) : environ -> mpred :=
@@ -28,29 +29,28 @@ Proof. intros. apply pred_ext.
 apply orp_left; apply derives_refl.
 apply orp_right1; apply derives_refl.
 Qed.
+Check mapsto_zeros.
 
-Lemma address_mapsto_zeros_memory_block:
- forall sh n b,
-  0 <= n <= Int.max_unsigned ->
-  address_mapsto_zeros sh (nat_of_Z n) (b, 0) |--
-  memory_block sh (Int.repr n) (Vptr b Int.zero).
+Lemma mapsto_zeros_memory_block:
+ forall sh n b ofs,
+  0 <= n ->
+  0 <= ofs ->
+  ofs+n <= Int.max_unsigned ->
+  mapsto_zeros n sh (Vptr b (Int.repr ofs)) |--
+  memory_block sh (Int.repr n) (Vptr b (Int.repr ofs)).
 Proof.
+ unfold mapsto_zeros.
 intros.
+ rename H0 into H'. rename H1 into H2.
 Transparent memory_block.
  unfold memory_block.
 Opaque memory_block.
- rewrite Int.unsigned_repr by auto.
-rewrite Int.unsigned_zero.
- assert (exists i, i=0) as [i ?] by eauto.
- rewrite <- H0.
- assert (0 <= i) by omega.
- assert (i + n <= Int.max_unsigned).
- subst. omega.
+repeat rewrite Int.unsigned_repr by omega.
  rewrite <- (Z2Nat.id n) in H2 by omega.
+ rewrite <- (Z2Nat.id n) in H by omega.
  change nat_of_Z with Z.to_nat.
- clear - H1 H2.
  forget (Z.to_nat n) as n'.
- revert i H1 H2;  induction n'; intros.
+ revert ofs H H' H2;  induction n'; intros.
  simpl; auto.
  rewrite inj_S in H2. unfold Z.succ in H2.
  apply sepcon_derives; auto.
@@ -61,23 +61,22 @@ rewrite Int.unsigned_zero.
  rewrite Int.unsigned_repr by omega. 
  auto.
  fold address_mapsto_zeros. fold memory_block'.
- apply IHn'. omega. omega.
+ apply IHn'. omega. omega. omega.
 Qed.
+
 
 Lemma tc_globalvar_sound:
   forall Delta i t gv idata rho, 
    (var_types Delta) ! i = None ->
    (glob_types Delta) ! i = Some (Global_var t) ->
-   no_attr_type t = true ->
    gvar_volatile gv = false ->
-   gvar_info gv = t ->
-   gvar_init gv = idata :: nil ->
-   gvar_readonly gv = false ->
-   sizeof t <= Int.max_unsigned ->
+   gvar_init gv = idata ->
    tc_environ Delta rho ->
-   globvar2pred(i, gv) rho |-- init_data2pred idata Ews (eval_var i t rho) rho.
+   globvar2pred(i, gv) rho |-- init_data_list2pred idata (readonly2share (gvar_readonly gv)) (eval_var i t rho) rho.
 Proof.
-intros until 1. intros ? Hno; intros.
+pose (H2:=True).
+pose (H4:=True).
+pose (H5:=True); intros.
 unfold globvar2pred.
 simpl.
 destruct H6 as [? [? [? ?]]].
@@ -88,10 +87,8 @@ rewrite H3; simpl.
 unfold eval_var.
 unfold Map.get. rewrite H10. rewrite H11.
 simpl. rewrite eqb_type_refl.
-rewrite H4.
 simpl.
 change (Share.splice extern_retainer Tsh) with Ews.
-rewrite sepcon_emp.
 auto.
 Qed.
 
@@ -101,72 +98,148 @@ Definition zero_of_type (t: type) : val :=
   | _ => Vint Int.zero
  end.
 
-Definition init_data2pred' (Delta: tycontext)  (d: init_data)  (sh: share) (id: ident)(ty: type) : environ -> mpred :=
+Definition init_data2pred' (Delta: tycontext)  (d: init_data)  (sh: share) (ty: type) (v: environ->val) : environ -> mpred :=
  match d with
-  | Init_int8 i => `(mapsto sh tuchar) (eval_var id ty) `(Vint (Int.zero_ext 8 i))
-  | Init_int16 i => `(mapsto sh tushort) (eval_var id ty) ` (Vint (Int.zero_ext 16 i))
-  | Init_int32 i => `(mapsto sh tuint) (eval_var id ty) ` (Vint i)
-  | Init_int64 i => `(mapsto sh tulong) (eval_var id ty) ` (Vlong i)
-  | Init_float32 r =>  `(mapsto sh tfloat) (eval_var id ty) ` (Vfloat ((Float.singleoffloat r)))
-  | Init_float64 r =>  `(mapsto sh tdouble) (eval_var id ty) ` (Vfloat r)
+  | Init_int8 i => `(mapsto sh tuchar) v `(Vint (Int.zero_ext 8 i))
+  | Init_int16 i => `(mapsto sh tushort) v ` (Vint (Int.zero_ext 16 i))
+  | Init_int32 i => `(mapsto sh tuint) v ` (Vint i)
+  | Init_int64 i => `(mapsto sh tulong) v ` (Vlong i)
+  | Init_float32 r =>  `(mapsto sh tfloat) v ` (Vfloat ((Float.singleoffloat r)))
+  | Init_float64 r =>  `(mapsto sh tdouble) v ` (Vfloat r)
   | Init_space n => 
-     if andb (Z.leb 0 n) (Z.leb n Int.max_unsigned)
-     then
       match ty  with
       | Tarray t j att => if zeq n (sizeof ty)
-                                  then `(array_at_ t sh 0 j) (eval_var id ty) (* FIXME *)
-                                  else `(memory_block sh (Int.repr n)) (eval_var id ty) 
+                                  then `(array_at_ t sh 0 j) v (* FIXME *)
+                                  else TT
       | Tvoid => TT
       | Tfunction _ _ => TT
       | Tstruct _ _ _ => TT (* FIXME *)
       | Tunion _ _ _ => TT (* FIXME *)
       | Tcomp_ptr _ _ => TT
       | t=> if zeq n (sizeof t) 
-                               then `(mapsto sh t) (eval_var id ty) `(zero_of_type t)
-                               else `(memory_block sh (Int.repr n)) (eval_var id ty) 
+                               then `(mapsto sh t) v `(zero_of_type t)
+                               else  TT
       end
-    else TT
   | Init_addrof symb ofs => 
       match (var_types Delta) ! symb, (glob_types Delta) ! symb with
-      | None, Some (Global_var (Tarray t _ att)) =>`(memory_block sh (Int.repr 4)) (eval_var id ty)
+      | None, Some (Global_var (Tarray t _ att)) =>`(memory_block sh (Int.repr 4)) v
       | None, Some (Global_var Tvoid) => TT
-      | None, Some (Global_var t) => `(mapsto sh (Tpointer t noattr)) (eval_var id ty) (`(offset_val ofs) (eval_var symb t))
-      | Some _, Some (Global_var (Tarray t _ att)) => `(memory_block sh (Int.repr 4)) (eval_var id ty)
+      | None, Some (Global_var t) => `(mapsto sh (Tpointer t noattr)) v (`(offset_val ofs) (eval_var symb t))
+      | Some _, Some (Global_var (Tarray t _ att)) => `(memory_block sh (Int.repr 4)) v
       | Some _, Some (Global_var Tvoid) => TT
-      | Some _, Some (Global_var t) => `(memory_block sh (Int.repr 4)) (eval_var id ty) 
+      | Some _, Some (Global_var t) => `(memory_block sh (Int.repr 4)) v 
       | _, _ => TT
       end
  end.
 
-
 Lemma mapsto_zeros_Tint:
-  forall i s a b,
-   mapsto_zeros (sizeof (Tint i s a)) Ews (Vptr b Int.zero)
-|-- mapsto Ews (Tint i s a) (Vptr b Int.zero) (Vint Int.zero).
+  forall sh i s a b ofs,
+   ofs + sizeof (Tint i s a) <= Int.max_unsigned ->
+   mapsto_zeros (sizeof (Tint i s a)) sh (Vptr b (Int.repr ofs))
+|-- mapsto sh (Tint i s a) (Vptr b (Int.repr ofs)) (Vint Int.zero).
 Admitted.
 
 Lemma mapsto_zeros_Tlong:
-  forall s a b,
-   mapsto_zeros (sizeof (Tlong s a)) Ews (Vptr b Int.zero)
-|-- mapsto Ews (Tlong s a) (Vptr b Int.zero) (Vint Int.zero).
+  forall sh s a b ofs,
+   ofs + sizeof (Tlong s a) <= Int.max_unsigned ->
+   mapsto_zeros (sizeof (Tlong s a)) sh (Vptr b (Int.repr ofs))
+|-- mapsto sh (Tlong s a) (Vptr b (Int.repr ofs)) (Vint Int.zero).
 Admitted.
 
 Lemma mapsto_zeros_Tfloat:
-  forall f a b, 
-  mapsto_zeros (sizeof (Tfloat f a)) Ews (Vptr b Int.zero)
-|-- mapsto Ews (Tfloat f a) (Vptr b Int.zero) (Vfloat Float.zero).
+  forall sh f a b ofs, 
+   ofs + sizeof (Tfloat f a) <= Int.max_unsigned ->
+  mapsto_zeros (sizeof (Tfloat f a)) sh (Vptr b (Int.repr ofs))
+|-- mapsto sh (Tfloat f a) (Vptr b (Int.repr ofs)) (Vfloat Float.zero).
 Admitted.
 
 Lemma mapsto_zeros_Tpointer:
-  forall t a b, 
-mapsto_zeros (sizeof (Tpointer t a)) Ews (Vptr b Int.zero)
-|-- mapsto Ews (Tpointer t a) (Vptr b Int.zero) (Vint Int.zero).
+  forall sh t a b ofs, 
+   ofs + sizeof (Tpointer t a) <= Int.max_unsigned ->
+mapsto_zeros (sizeof (Tpointer t a)) sh (Vptr b (Int.repr ofs))
+|-- mapsto sh (Tpointer t a) (Vptr b (Int.repr ofs)) (Vint Int.zero).
 Admitted.
 
 Lemma unpack_globvar_aux1:
-  forall sh t a b v, umapsto sh (Tpointer t a) (Vptr b Int.zero) v
-                   |-- memory_block sh (Int.repr 4) (Vptr b Int.zero).
+  forall sh t a b v ofs, 
+   ofs + sizeof (Tpointer t a) <= Int.max_unsigned ->
+               umapsto sh (Tpointer t a) (Vptr b (Int.repr ofs)) v
+                   |-- memory_block sh (Int.repr 4) (Vptr b (Int.repr ofs)).
 Admitted.
+
+Lemma sizeof_Tpointer: forall t a, sizeof (Tpointer t a) = 4.
+Proof.
+(* NOt quite true in CompCert 2.1, if the attributes a contain "align_as".
+But it will be true again in CompCert 2.2.
+*)
+Admitted.
+
+Lemma init_data_size_space:
+ forall t, init_data_size (Init_space (sizeof t)) = sizeof t.
+Proof. intros.
+ pose proof (sizeof_pos t).
+ simpl. rewrite Z.max_l; auto. omega.
+Qed.
+
+Lemma init_data2pred_rejigger:
+  forall (Delta : tycontext) (t : type) (idata : init_data) (rho : environ)
+     (sh : Share.t) (b : block) ofs (v : environ -> val),
+  no_attr_type t = true ->
+  0 <= ofs ->
+  ofs + init_data_size idata <= Int.max_unsigned ->
+  tc_environ Delta rho ->
+  v rho = Vptr b (Int.repr 0) ->
+   init_data2pred idata sh (offset_val (Int.repr ofs) (v rho)) rho 
+    |-- init_data2pred' Delta idata sh t (`(offset_val (Int.repr ofs)) v) rho.
+Proof.
+intros until v.
+intros H1 H6' H6 H7 H8.
+ unfold init_data2pred', init_data2pred.
+ rename H8 into H8'.
+ assert (H8: offset_val (Int.repr ofs) (v rho) = Vptr b (Int.repr ofs)).
+ rewrite H8'; simpl. rewrite Int.add_zero_l; auto.
+ clear H8'.
+ destruct idata; super_unfold_lift;
+ try solve [apply andp_right; [apply prop_right; apply I | apply derives_refl]].
+*  
+ destruct t; try (apply no_attr_e in H1; subst a);
+  try (simpl; apply TT_right);
+  try (if_tac;
+        [rewrite H8; unfold zero_of_type; subst z; 
+         rewrite init_data_size_space in H6
+        | simpl; apply TT_right
+        ]).
++ apply mapsto_zeros_Tint; auto.
++ apply mapsto_zeros_Tlong; auto.
++ apply mapsto_zeros_Tfloat; auto.
++ apply mapsto_zeros_Tpointer; auto.
++  eapply derives_trans; [ apply mapsto_zeros_memory_block; try omega | ].
+pose proof (sizeof_pos (Tarray t z0 a)); omega.
+ rewrite memory_block_typed by assumption.
+ rewrite array_at_arrayof'.
+ unfold typed_mapsto_. simpl.
+ rewrite withspacer_spacer. unfold spacer. rewrite align_0. simpl.
+ rewrite emp_sepcon.
+ rewrite Z.mul_0_r. rewrite Z.sub_0_r.
+ apply derives_refl.
+ apply alignof_pos.
+*  (*simpl in H5.*)
+   destruct ((var_types Delta) ! i) eqn:Hv;
+   destruct ((glob_types Delta) ! i) eqn:Hg; 
+    try destruct g; try solve [simpl; apply TT_right].
+ +
+    destruct (proj1 (proj2 (proj2 H7)) _ _ Hg) as [b' [H15 H16]]; rewrite H15.
+    rewrite H8. (*clear dependent i. *)
+    destruct gv; simpl; try apply TT_right; try rewrite H8;
+     try  apply unpack_globvar_aux1; rewrite sizeof_Tpointer; simpl in H6; omega.
+ + 
+    destruct (proj1 (proj2 (proj2 H7)) _ _ Hg) as [b' [H15 H16]]; rewrite H15.
+    assert (eval_var i gv rho = Vptr b' Int.zero)
+      by admit.  (* straightforward *) 
+    destruct gv; simpl; try apply TT_right; try rewrite H8; try rewrite H;
+    unfold mapsto; try (apply andp_right; [apply prop_right; apply I | apply derives_refl ]).
+apply unpack_globvar_aux1; rewrite sizeof_Tpointer; simpl in H6; omega.
+Qed.
 
 Lemma unpack_globvar:
   forall Delta i t gv idata, 
@@ -176,57 +249,81 @@ Lemma unpack_globvar:
    gvar_volatile gv = false ->
    gvar_info gv = t ->
    gvar_init gv = idata :: nil ->
-   gvar_readonly gv = false ->
-   sizeof t <= Int.max_unsigned ->
+   init_data_size idata <= sizeof t ->
+   sizeof t <= Int.max_unsigned ->  
    local (tc_environ Delta) && globvar2pred(i, gv) |-- 
-       init_data2pred' Delta idata Ews i t.
+       init_data2pred' Delta idata (Share.splice extern_retainer (readonly2share (gvar_readonly gv))) t (eval_var i t).
 Proof.
 intros.
 go_lowerx.
-eapply derives_trans; [eapply tc_globalvar_sound; eassumption | ].
+eapply derives_trans; [eapply tc_globalvar_sound; try eassumption | ].
+forget (readonly2share (gvar_readonly gv)) as sh.
+unfold init_data_list2pred.
+simpl.
+rewrite sepcon_emp.
 destruct (tc_eval_gvar_zero _ _ _ _ H7 H H0) as [b ?].
- unfold init_data2pred', init_data2pred.
- destruct idata; super_unfold_lift;
- try solve [apply andp_right; [apply prop_right; apply I | apply derives_refl]].
- destruct (0 <=? z) eqn:? ; [ | simpl; apply TT_right].
- destruct (z <=? Int.max_unsigned) eqn:? ; [ | simpl; apply TT_right].
- apply Zle_bool_imp_le in Heqb0.
- apply Zle_bool_imp_le in Heqb1.
-* destruct t;
-  try (simpl; apply TT_right);
-  try (simpl andb; cbv iota; if_tac;
-        [rewrite H8; unfold zero_of_type; subst z;
-         first [simple apply mapsto_zeros_Tint | simple apply mapsto_zeros_Tlong 
-                |simple apply mapsto_zeros_Tfloat | simple apply mapsto_zeros_Tpointer
-                ]
-        | rewrite H8; apply address_mapsto_zeros_memory_block; split; auto
-        ]).
- + simpl andb; cbv iota; if_tac; rewrite H8.
-   eapply derives_trans; [ apply address_mapsto_zeros_memory_block; split; auto | ].
-   subst z.
- rewrite memory_block_typed.
- rewrite array_at_arrayof'.
- unfold typed_mapsto_. simpl.
- rewrite withspacer_spacer. unfold spacer. rewrite align_0. simpl.
- rewrite emp_sepcon.
- rewrite Z.mul_0_r. rewrite Z.sub_0_r.
- apply derives_refl.
- apply alignof_pos.
- apply H1.
- apply address_mapsto_zeros_memory_block; split; auto.
-* destruct ((var_types Delta) ! i0) eqn:Hv;
-   destruct ((glob_types Delta) ! i0) eqn:Hg; 
-    try destruct g; try solve [simpl; apply TT_right].
- destruct (proj1 (proj2 (proj2 H7)) _ _ Hg) as [b' [H15 H16]]; rewrite H15.
-  rewrite H8.
- destruct gv0; simpl; try apply TT_right; try rewrite H8;
-   try  apply unpack_globvar_aux1.
-  destruct (proj1 (proj2 (proj2 H7)) _ _ Hg) as [b' [H15 H16]]; rewrite H15.
- assert (eval_var i0 gv0 rho = Vptr b' Int.zero)
-   by admit.  (* straightforward *)
- destruct gv0; simpl; try apply TT_right; try rewrite H8; try rewrite H9;
- unfold mapsto; try (apply andp_right; [apply prop_right; apply I | apply derives_refl ]).
-apply unpack_globvar_aux1.
+ replace (eval_var i t rho) with (offset_val Int.zero (eval_var i t rho)) by (rewrite H8; reflexivity).
+ eapply derives_trans; [eapply init_data2pred_rejigger; eauto; omega | ].
+ unfold init_data2pred'.
+ destruct idata; unfold_lift; try destruct t; try if_tac;
+   try (rewrite H8; simpl; rewrite Int.add_zero_l; auto);
+ try apply derives_refl;
+ destruct ( (glob_types Delta) ! i0); try destruct g;try destruct gv0; try apply derives_refl;
+   try (rewrite H8; simpl; rewrite Int.add_zero_l; auto).
+Qed.
+
+Fixpoint id2pred_star (Delta: tycontext) (sh: share) (t: type) (v: environ->val) (ofs: Z) (dl: list init_data) : environ->mpred :=
+ match dl with
+ | d::dl' => init_data2pred' Delta d sh t (`(offset_val (Int.repr ofs)) v)
+                   * id2pred_star Delta sh t v (ofs + init_data_size d) dl'
+ | nil => emp
+ end.
+
+Lemma init_data_list_size_pos : forall a, init_data_list_size a >= 0.
+Admitted.
+
+Lemma init_data_size_pos : forall a, init_data_size a > 0.
+Admitted.
+
+
+Lemma unpack_globvar_star:
+  forall Delta i gv, 
+   (var_types Delta) ! i = None ->
+   (glob_types Delta) ! i = Some (Global_var (gvar_info gv)) ->
+   no_attr_type (gvar_info gv) = true ->
+   gvar_volatile gv = false ->
+   gvar_readonly gv = false ->
+   init_data_list_size (gvar_init gv) <= sizeof (gvar_info gv) <= Int.max_unsigned ->
+   local (tc_environ Delta) && globvar2pred(i, gv) |-- 
+       id2pred_star Delta (Share.splice extern_retainer (readonly2share (gvar_readonly gv))) (gvar_info gv) (eval_var i (gvar_info gv)) 0 (gvar_init gv).
+Proof.
+intros until 4.
+remember (gvar_info gv) as t eqn:H3; symmetry in H3.
+remember (gvar_init gv) as idata eqn:H4; symmetry in H4.
+intros. 
+go_lowerx.
+eapply derives_trans; [eapply tc_globalvar_sound; eassumption | ].
+forget (readonly2share (gvar_readonly gv)) as sh.
+destruct (tc_eval_gvar_zero _ _ _ _ H7 H H0) as [b ?].
+set (ofs:=0%Z).
+replace (eval_var i t rho) with (offset_val (Int.repr ofs) (eval_var i t rho))
+   by (rewrite H8; reflexivity).
+assert (H11: init_data_list_size idata + ofs <= sizeof t)  by (unfold ofs; omega).
+assert (H12:  sizeof t <= Int.max_unsigned)  by omega.
+assert (0 <= ofs) by (unfold ofs; omega).
+clearbody ofs.
+revert ofs H9 H11 H12.
+clear dependent gv. clear H H0 H6.
+induction idata; simpl; auto; intros.
+apply sepcon_derives.
+* eapply init_data2pred_rejigger; eauto.
+ pose proof (init_data_list_size_pos idata); omega.
+* specialize (IHidata (ofs + init_data_size a)).
+rewrite offset_offset_val.
+rewrite add_repr.
+ pose proof (init_data_list_size_pos idata).
+pose proof (init_data_size_pos a).
+ apply IHidata; try omega.
 Qed.
 
 Lemma tc_globalvar_sound_space:
@@ -249,31 +346,114 @@ simpl.
 rewrite <- memory_block_typed by auto.
 destruct (tc_eval_gvar_zero _ _ _ _ H6 H H0) as [b ?].
 rewrite H7.
-unfold mapsto_zeros.
+unfold mapsto_zeros. rewrite sepcon_emp.
 rewrite Int.unsigned_zero.
-apply address_mapsto_zeros_memory_block.
-pose (sizeof_pos t); omega.
+pose proof (mapsto_zeros_memory_block Ews (sizeof t) b 0).
+unfold mapsto_zeros in H8. change (Int.repr 0) with Int.zero in H8.
+rewrite Int.unsigned_zero in H8. rewrite H4. apply H8.
+pose (sizeof_pos t); omega. omega. omega.
 Qed.
 
-(*
-Lemma tc_globalvar_sound':
-  forall Delta i t gv, 
-   (var_types Delta) ! i = None ->
-   (glob_types Delta) ! i = Some (Global_var t) ->
-   no_attr_type t = true ->
-   gvar_volatile gv = false ->
-   gvar_info gv = t ->
-   gvar_init gv = Init_space (sizeof t) :: nil ->
-   gvar_readonly gv = false ->
-   sizeof t <= Int.max_unsigned ->
-   local (tc_environ Delta) && globvar2pred(i, gv) |-- 
-   `(typed_mapsto_ Ews t) (eval_var i t).
-Proof.
-intros.
-go_lowerx.
-eapply tc_globalvar_sound; eauto.
+Lemma array_at_emp:
+ forall t sh f lo v, array_at t sh f lo lo v = emp.
+Proof. intros. unfold array_at, rangespec.
+replace (lo-lo) with 0 by omega.
+simpl. auto.
 Qed.
-*) 
+
+Lemma idpred2_star_ZnthV_tint:
+ forall Delta sh n v (data: list int) mdata,
+  n = Zlength mdata ->
+  mdata = map Init_int32 data ->
+  id2pred_star Delta sh (tarray tint n) v 0 mdata |--
+  `(array_at tint sh (ZnthV tint data) 0 n) v.
+Proof.
+intros. subst n mdata.
+replace (Zlength (map Init_int32 data)) with (Zlength data)
+ by (repeat rewrite Zlength_correct; rewrite map_length; auto).
+go_lowerx.
+set (ofs:=0%Z).
+unfold ofs at 1.
+change 0 with (ofs*4)%Z.
+set (N := Zlength data). unfold N at 2. clearbody N.
+replace (Zlength data) with (ofs + Zlength data) by (unfold ofs; omega).
+replace (ZnthV tint data) with (fun i => ZnthV tint data (i-ofs))
+  by (extensionality i; unfold ofs; rewrite Z.sub_0_r; auto).
+clearbody ofs.
+
+revert ofs;
+induction data; intros; simpl; auto.
+* rewrite Zlength_nil. unfold array_at, rangespec; simpl.
+ replace (ofs+0-ofs) with 0 by omega. simpl. auto.
+* rewrite Zlength_cons.
+replace (ofs*4+4) with ((Z.succ ofs) * 4)%Z 
+ by (unfold Z.succ; rewrite Z.mul_add_distr_r; reflexivity).
+replace (ofs + Z.succ (Zlength data)) with (Z.succ ofs + Zlength data) by omega.
+rewrite (split3_array_at ofs).
+rewrite array_at_emp. rewrite emp_sepcon.
+apply sepcon_derives; auto.
+unfold_lift.
+change (mapsto sh tuint (offset_val (Int.repr (ofs * 4)) (v rho)) (Vint a))
+ with (mapsto sh tint (offset_val (Int.repr (ofs * 4)) (v rho)) (Vint a)).
+pose proof (typed_mapsto_tint sh (`(offset_val (Int.repr (ofs*4))) v) (`a)).
+match type of H with (?A = ?B) => assert (A rho = B rho) by (apply f_equal; auto) end.
+unfold_lift in H0.  unfold_lift.
+rewrite mapsto_isptr.
+apply derives_extract_prop. intro.
+destruct (v rho); inv H1.
+rewrite <- H0.
+unfold add_ptr_int; simpl.
+rewrite mul_repr.
+unfold ZnthV.
+change (align 4 4) with 4.
+rewrite Zmult_comm.
+unfold typed_mapsto_opt.
+if_tac.
+auto with cancel.
+rewrite Z.sub_diag. simpl nth_error. unfold value.
+auto.
+eapply derives_trans; [ apply IHdata | ].
+apply derives_refl'.
+apply equal_f. apply array_at_ext.
+intros. unfold ZnthV. if_tac. rewrite if_true by omega. auto.
+rewrite if_false by omega.
+assert (Z.to_nat (i-ofs) = S (Z.to_nat (i - Z.succ ofs))).
+apply Nat2Z.inj. rewrite inj_S. rewrite Z2Nat.id by omega.
+rewrite Z2Nat.id by omega. omega.
+rewrite H1. simpl. auto.
+rewrite Zlength_correct; clear; omega.
+Qed.
+
+
+Lemma map_instantiate:
+  forall {A B} (f: A -> B) (x: A) (y: list B) z,
+    y = map f z ->  f x :: y = map f (x :: z).
+Proof. intros. subst. reflexivity. Qed.
+
+
+Lemma unpack_globvar_array:
+  forall data n Delta i gv, 
+   (var_types Delta) ! i = None ->
+   (glob_types Delta) ! i = Some (Global_var (gvar_info gv)) ->
+   gvar_info gv = tarray tint n ->
+   gvar_volatile gv = false ->
+   gvar_readonly gv = false ->
+   n = Zlength (gvar_init gv) ->
+   gvar_init gv = map Init_int32 data ->
+   init_data_list_size (gvar_init gv) <= sizeof (gvar_info gv) <= Int.max_unsigned ->
+   local (tc_environ Delta) && globvar2pred(i, gv) |-- 
+      `(array_at tint (Share.splice extern_retainer (readonly2share (gvar_readonly gv)))
+    (ZnthV tint data) 0 n) (eval_var i (tarray tint n)).
+Proof.
+ intros.
+ eapply derives_trans.
+ apply unpack_globvar_star; try eassumption; try reflexivity.
+ rewrite H1; reflexivity.
+ rewrite H1. rewrite H3. rewrite H5.
+ change (Share.splice extern_retainer (readonly2share false)) with Ews. 
+ apply idpred2_star_ZnthV_tint; auto.
+ rewrite <- H5. auto.
+Qed.
 
 Lemma main_pre_eq:
  forall prog u, main_pre prog u = 
@@ -329,6 +509,11 @@ first [
     eapply unpack_globvar;
       [reflexivity | reflexivity | reflexivity | reflexivity | reflexivity | reflexivity
       | reflexivity | compute; congruence ]
+ | eapply unpack_globvar_array;
+      [reflexivity | reflexivity | reflexivity | reflexivity | reflexivity
+      | compute; clear; congruence 
+      | repeat eapply map_instantiate; symmetry; apply map_nil
+      | compute; split; clear; congruence ]
  | apply andp_left2; apply derives_refl
  ].
 
